theories/TM/L/CompilerBoolFuns/Compiler_spec.v
@@ -5,29 +5,29 @@ From Undecidability.TM Require Import TM Util.TM_facts.
 
 Import ListNotations Vector.VectorNotations.
 
-Definition encListTM {Σ : Type} (s b : Σ) (l : list bool) :=
+Definition encBoolsListTM {Σ : Type} (s b : Σ) (l : list bool) :=
   (map (fun (x : bool) => (if x then s else b)) l).
 
-Definition encTM {Σ : Type} (s b : Σ) (l : list bool) :=
-  @midtape Σ [] b (encListTM s b l).
+Definition encBoolsTM {Σ : Type} (s b : Σ) (l : list bool) :=
+  @midtape Σ [] b (encBoolsListTM s b l).
 
   
 Definition TM_booL_bool_computable {k} (R : Vector.t (list bool) k -> (list bool) -> Prop) := 
   exists n : nat, exists Σ : finType, exists s b : Σ, s <> b /\ 
   exists M : TM Σ (k + 1 + n),
   forall v : Vector.t (list bool) k, 
-  (forall m, R v m <-> exists q t, TM.eval M (start M) ((Vector.map (encTM s b) v ++ [niltape]) ++ Vector.const niltape n) q t
-                                /\ nth_error (Vector.to_list t) k = Some (encTM s b m)) /\
-  (forall q t, TM.eval M (start M) ((Vector.map (encTM s b) v ++ [niltape]) ++ Vector.const niltape n) q t ->
-          exists m, nth_error (Vector.to_list t) k = Some (encTM s b m)).
+  (forall m, R v m <-> exists q t, TM.eval M (start M) ((Vector.map (encBoolsTM s b) v ++ [niltape]) ++ Vector.const niltape n) q t
+                                /\ nth_error (Vector.to_list t) k = Some (encBoolsTM s b m)) /\
+  (forall q t, TM.eval M (start M) ((Vector.map (encBoolsTM s b) v ++ [niltape]) ++ Vector.const niltape n) q t ->
+          exists m, nth_error (Vector.to_list t) k = Some (encBoolsTM s b m)).
 
 Definition TM₁_booL_bool_computable {k} (Σ : finType) (R : Vector.t (list bool) k -> (list bool) -> Prop) := 
   exists s1 s2 b : Σ, s1 <> s2 /\ s1 <> b /\ s2 <> b /\
   exists M : TM Σ 1,
   forall v : Vector.t (list bool) k, 
-  (forall m, R v m <-> exists q, TM.eval M (start M) [midtape [] b (Vector.fold_right (fun l s => encListTM s1 s2 l ++ s)%list v List.nil)] q [encTM s1 s2 m]) /\
-  (forall q t, TM.eval M (start M) [midtape [] b (Vector.fold_right (fun l s => encListTM s1 s2 l ++ s)%list v List.nil)] q t ->
-          exists m, t = [encTM s1 s2 m]).
+  (forall m, R v m <-> exists q, TM.eval M (start M) [midtape [] b (Vector.fold_right (fun l s => encBoolsListTM s1 s2 l ++ s)%list v List.nil)] q [encBoolsTM s1 s2 m]) /\
+  (forall q t, TM.eval M (start M) [midtape [] b (Vector.fold_right (fun l s => encBoolsListTM s1 s2 l ++ s)%list v List.nil)] q t ->
+          exists m, t = [encBoolsTM s1 s2 m]).
       
 Definition encL (l : list bool) := list_enc l.
 
